CertiGC/verif_do_scan.v
@@ -5,13 +5,15 @@ Lemma body_do_scan: semax_body Vprog Gprog f_do_scan do_scan_spec.
 Proof.
   start_function.
   forward.
-  forward_loop (EX index: nat, EX g': LGraph, EX t_info': thread_info,
+  forward_loop (EX n: nat, EX g': LGraph, EX t_info': thread_info,
                 PROP (super_compatible (g', t_info', roots) f_info outlier;
                       forward_condition g' t_info' from to;
                       thread_info_relation t_info t_info';
-                      closure_has_index g' to index)
+                      closure_has_index g' to (to_index + n);
+                      scan_vertex_while_loop from to (nat_seq to_index n) g g')
                 LOCAL
-                (temp _s (offset_val (- WORD_SIZE) (vertex_address g' (to, index)));
+                (temp _s (offset_val (- WORD_SIZE)
+                                     (vertex_address g' (to, (to_index + n)%nat)));
                  temp _from_start (gen_start g' from);
                  temp _from_limit (limit_address g' t_info' from);
                  temp _next (next_address t_info' to))
@@ -25,17 +27,20 @@ Proof.
           LOCAL ()
           SEP (all_string_constants rsh gv; outlier_rep outlier;
                graph_rep g'; thread_info_rep sh t_info' ti)).
-  - Exists to_index g t_info. destruct H as [? [? [? ?]]]. entailer!. apply tir_id.
-  - Intros index g' t_info'. unfold next_address, thread_info_rep. Intros.
+  - Exists O g t_info. destruct H as [? [? [? ?]]].
+    replace (to_index + 0)%nat with to_index by omega. entailer!.
+    split; [apply tir_id | constructor].
+  - Intros n g' t_info'. remember (to_index + n)%nat as index.
+    unfold next_address, thread_info_rep. Intros.
     unfold heap_struct_rep. destruct H5 as [? [? [? ?]]].
     destruct H6 as [? [? [? [? ?]]]].
     assert (0 <= Z.of_nat to < 12). {
-      clear -H5 H13. destruct H5 as [_ [_ ?]]. red in H13.
+      clear -H5 H14. destruct H5 as [_ [_ ?]]. red in H14.
       pose proof (spaces_size (ti_heap t_info')).
       rewrite Zlength_correct in H0. rep_omega. } assert (0 < Z.of_nat to) by omega.
-    destruct (gt_gs_compatible _ _ H5 _ H13) as [? [? ?]]. rewrite nth_space_Znth in *.
+    destruct (gt_gs_compatible _ _ H5 _ H14) as [? [? ?]]. rewrite nth_space_Znth in *.
     remember (Znth (Z.of_nat to) (spaces (ti_heap t_info'))) as sp_to.
-    assert (isptr (space_start sp_to)) by (rewrite <- H18; apply start_isptr).
+    assert (isptr (space_start sp_to)) by (rewrite <- H19; apply start_isptr).
     remember ((space_start (heap_head (ti_heap t_info')),
                (Vundef,
                 offset_val (WORD_SIZE * total_space (heap_head (ti_heap t_info')))
@@ -46,13 +51,13 @@ Proof.
       rewrite map_tl, Znth_tl by omega.
       replace (Z.of_nat to - 1 + 1) with (Z.of_nat to) by omega.
       rewrite Znth_map by (rewrite spaces_size; rep_omega). reflexivity. }
-    unfold Inhabitant_pair, Inhabitant_val, Inhabitant in H22.
-    forward; rewrite H22; unfold space_tri. 1: entailer!.
+    unfold Inhabitant_pair, Inhabitant_val, Inhabitant in H23.
+    forward; rewrite H23; unfold space_tri. 1: entailer!.
     unfold vertex_address, vertex_offset. rewrite offset_offset_val. simpl vgeneration.
     simpl vindex.
     replace (WORD_SIZE * (previous_vertices_size g' to index + 1) + - WORD_SIZE) with
         (WORD_SIZE * (previous_vertices_size g' to index))%Z by rep_omega.
-    unfold gen_start at 1. rewrite if_true by assumption. rewrite H18.
+    unfold gen_start at 1. rewrite if_true by assumption. rewrite H19.
     remember (WORD_SIZE * used_space sp_to)%Z as used_offset.
     remember (WORD_SIZE * previous_vertices_size g' to index)%Z as index_offset.
     freeze [0; 1; 3; 4] FR. gather_SEP 1 2.
@@ -61,21 +66,22 @@ Proof.
           Vptr b i = space_start sp_to ->
           graph_rep g' * heap_rest_rep (ti_heap t_info') |--
       !! (WORD_SIZE * total_space sp_to + Ptrofs.unsigned i <= Ptrofs.max_unsigned)). {
-      intros. sep_apply (graph_and_heap_rest_data_at_ _ _ _ H13 H5).
+      intros. sep_apply (graph_and_heap_rest_data_at_ _ _ _ H14 H5).
       assert (space_start sp_to = gen_start g' to) by
           (unfold gen_start; rewrite if_true by assumption;
-           rewrite <- H18; reflexivity). rewrite H24 in H23.
-      sep_apply (generation_data_at__ptrofs g' t_info' to b i H23). entailer!.
-      unfold gen_size in H25. rewrite nth_space_Znth in H25. assumption. }
-    forward_if (gen_has_index g' to index). 
+           rewrite <- H19; reflexivity). rewrite H25 in H24.
+      sep_apply (generation_data_at__ptrofs g' t_info' to b i H24). entailer!.
+      unfold gen_size in H26. rewrite nth_space_Znth in H26. assumption. }
+    forward_if (gen_has_index g' to index).
     + remember (Znth (Z.of_nat to) (spaces (ti_heap t_info'))) as sp_to.
-      sep_apply (graph_and_heap_rest_data_at_ _ _ _ H13 H5).
+      sep_apply (graph_and_heap_rest_data_at_ _ _ _ H14 H5).
       unfold generation_data_at_.
       assert (gen_start g' to = space_start sp_to) by
-          (subst; unfold gen_start; rewrite if_true; assumption). rewrite H30.
+          (subst; unfold gen_start; rewrite if_true; assumption). rewrite H31.
       rewrite data_at__memory_block. Intros. rewrite sizeof_tarray_int_or_ptr.
       2: unfold gen_size; apply (proj1 (total_space_range (nth_space t_info' to))).
       remember (WORD_SIZE * used_space sp_to)%Z as used_offset.
+      remember (to_index + n)%nat as index.
       remember (WORD_SIZE * previous_vertices_size g' to index)%Z as index_offset.
       destruct (space_start sp_to); try contradiction. simpl. unfold test_order_ptrs.
       simpl. case (peq b b); intros. 2: contradiction. simpl.
@@ -92,42 +98,43 @@ Proof.
         sep_apply (memory_block_weak_valid_pointer
                      (nth_sh g' to) (WORD_SIZE * gen_size t_info' to)
                      (Vptr b i) offset); auto. 3: apply extend_weak_valid_pointer.
-        - subst. unfold gen_size. split. 1: apply (proj1 H33).
+        - subst. unfold gen_size. split. 1: apply (proj1 H34).
           transitivity (WORD_SIZE * used_space (nth_space t_info' to))%Z.
-          + rewrite nth_space_Znth. apply (proj2 H33).
+          + rewrite nth_space_Znth. apply (proj2 H34).
           + apply Zmult_le_compat_l. apply (proj2 (space_order _)). rep_omega.
         - unfold gen_size. clear -H4 H7. destruct H7. unfold gen_size in H0.
           rewrite <- H0. rewrite nth_space_Znth. rep_omega. }
-      apply andp_right; apply H33.
-      * subst. split. 1: pose proof (pvs_ge_zero g' to index); rep_omega.
-        apply Zmult_le_compat_l. 2: rep_omega. rewrite <- H20.
+      apply andp_right; apply H34.
+      * subst. split. 1: pose proof (pvs_ge_zero g' to (to_index + n)%nat); rep_omega.
+        apply Zmult_le_compat_l. 2: rep_omega. rewrite <- H21.
         apply pvs_mono. assumption.
       * split. 2: omega. subst. apply Z.mul_nonneg_nonneg. 1: rep_omega.
         apply (proj1 (space_order _)).
     + assert_PROP (index_offset < used_offset). {
         remember (space_start sp_to). destruct v; try contradiction. inv_int i.
-        specialize (H23 b (Ptrofs.repr ofs) eq_refl).
-        rewrite Ptrofs.unsigned_repr in H23 by rep_omega. sep_apply H23. Intros.
+        specialize (H24 b (Ptrofs.repr ofs) eq_refl).
+        rewrite Ptrofs.unsigned_repr in H24 by rep_omega. sep_apply H24. Intros.
         assert (0 <= ofs + used_offset <= Ptrofs.max_unsigned). {
           subst. pose proof
                       (space_order (Znth (Z.of_nat to) (spaces (ti_heap t_info')))).
           rep_omega. }
         assert (0 <= ofs + index_offset <= Ptrofs.max_unsigned). {
-          subst. red in H8. pose proof (pvs_ge_zero g' to index).
+          subst. red in H8. pose proof (pvs_ge_zero g' to (to_index + n)%nat).
           pose proof (pvs_mono g' to _ _ H8). rep_omega. }
-        rewrite force_sem_cmp_pp in H24; [|rewrite isptr_offset_val; assumption..].
-        simpl in H24. rewrite !ptrofs_add_repr in H24.
-        rewrite if_true in H24. 2: reflexivity. unfold typed_true in H24.
+        rewrite force_sem_cmp_pp in H25; [|rewrite isptr_offset_val; assumption..].
+        simpl in H25. rewrite !ptrofs_add_repr in H25.
+        rewrite if_true in H25. 2: reflexivity. unfold typed_true in H25.
         destruct (Ptrofs.ltu (Ptrofs.repr (ofs + index_offset))
-                             (Ptrofs.repr (ofs + used_offset))) eqn: ?; simpl in H24.
-        2: inversion H24. unfold Ptrofs.ltu in Heqb0.
+                             (Ptrofs.repr (ofs + used_offset))) eqn: ?; simpl in H25.
+        2: inversion H25. unfold Ptrofs.ltu in Heqb0.
         rewrite !Ptrofs.unsigned_repr in Heqb0; auto.
         if_tac in Heqb0. 1: apply prop_right; omega. inversion Heqb0. }
-      forward. entailer!. red. rewrite <- H20 in H25.
-      rewrite <- Z.mul_lt_mono_pos_l in H25 by rep_omega.
-      apply pvs_lt_rev in H25. assumption.
+      forward. entailer!. red. rewrite <- H21 in H26.
+      rewrite <- Z.mul_lt_mono_pos_l in H26 by rep_omega.
+      apply pvs_lt_rev in H26. assumption.
     + forward. thaw FR. unfold thread_info_rep, heap_struct_rep.
-      Exists g' t_info'. unfold forward_condition. entailer!. admit.
+      Exists g' t_info'. unfold forward_condition. entailer!. exists n. split.
+      1: assumption. admit.
     + admit.
   - Intros g' t_info'. forward. Exists g' t_info'. entailer!.
 Abort.
